steel/Veritas.Formats.fsti
@@ -1,0 +1,35 @@
+module Veritas.Formats
+include Veritas.Formats.Pure
+
+module U8 = FStar.UInt8
+module U32 = FStar.UInt32
+module A = Steel.Array
+
+open Steel.Effect.Common
+open Steel.Effect
+
+val serialize_value: v:value -> dst: A.array U8.t { A.length dst == U32.v (serialize_length v) } ->
+  SteelT unit
+    (A.varray dst)
+    (fun _ -> A.varray dst)
+
+val extract_log_entry_from (len: U32.t) (buf: A.array U8.t { A.length buf == U32.v len }) (pos: A.array (x: U32.t { U32.v x <= U32.v len }) { A.length pos == 1 })
+  : SteelT (option vlog_entry)
+    (A.varray buf `star` A.varray pos)
+    (fun _ -> A.varray buf `star` A.varray pos)
+ (* /\
+            log at position h0.pos contains a vali repr of v *)
+
+val serialize_stamped_record
+  (dst: A.array U8.t { 184 <= A.length dst })
+  (r: stamped_record)
+: Steel U32.t
+  (A.varray dst)
+  (fun _ -> A.varray dst)
+  (fun _ -> True)
+  (fun h len h' ->
+    let s = h (A.varray dst) in
+    let s' = h' (A.varray dst) in
+    U32.v len <= A.length dst /\
+    Seq.slice s' (U32.v len) (Seq.length s') == Seq.slice s (U32.v len) (Seq.length s)
+  )
