steel/formats/Veritas.Formats.Pure.fsti
@@ -1,0 +1,7 @@
+module Veritas.Formats.Pure
+include Veritas.Formats.Aux
+include Veritas.Formats.Types
+
+module U32 = FStar.UInt32
+
+val serialize_length : value -> (l: U32.t { U32.v l > 0 })
