steel/formats/everparse/Veritas.Formats.Pure.fst
@@ -1,0 +1,5 @@
+module Veritas.Formats.Pure
+module LP = LowParse.Spec.Base
+
+let serialize_length x =
+  Veritas.Formats.EverParse.Value.value_size32 x
