steel/formats/everparse/Veritas.Formats.fsti
@@ -1,21 +1,11 @@
 module Veritas.Formats
-include Veritas.Formats.Aux
+include Veritas.Formats.Pure
 include Veritas.Formats.Types
 
 module U8 = FStar.UInt8
 module U32 = FStar.UInt32
 module HST = FStar.HyperStack.ST
 module B = LowStar.Buffer
-
-let bool_of_vbool (x: vbool) : Tot bool =
-  match x with
-  | Vfalse -> false
-  | Vtrue -> true
-
-let vbool_of_bool (x: bool) : Tot vbool =
-  if x then Vtrue else Vfalse
-
-val serialize_length : value -> (l: U32.t { U32.v l > 0 })
 
 val serialize_value: v:value -> dst: B.lbuffer U8.t (U32.v (serialize_length v)) ->
   HST.Stack unit
